Updated 2.4

Exercises 7/24_exercise_sheet.lean
@@ -1,2 +1,194 @@
-/- Lecture 2.4: Custom Tactics -/
+/- Exercise 2.4: Functional Programming — Metaprogramming -/
 
+open expr
+open tactic
+
+
+/- Question 1: A term exploder -/
+
+/- In this exercise, we develop a string format for the `expr` metatype. By default, there is no
+`has_repr` instance to print a nice string. For example: -/
+
+#eval (expr.app (expr.var 0) (expr.var 1) : expr)  -- result: `[external]`
+#eval (`(λx : ℕ, x + x) : expr)  -- result: `[external]`
+
+/- 1.1. Define a metafunction `expr.repr` that converts an `expr` into a `string`. It is acceptable
+to leave out some fields from the `expr` constructors, such as the level `l` of a sort, the binder
+information `bi` of a λ- or Π- binder, and the arguments of the `macro` constructor.
+
+Hint: Use `name.to_string` to convert a name to a string, and `repr` for other types that belong to
+the `has_repr` type class. -/
+
+-- enter your definition here
+
+/- 1.2. Register `expr.repr` in the `has_repr` type class, so that we can use `repr` without
+qualification in the future, and so that it is available to `#eval`.
+
+Hint: You will need the `meta` keyword in front of the command you enter. -/
+
+-- enter your command here
+
+/- 1.3. Test your setup. -/
+
+#eval (expr.app (expr.var 0) (expr.var 1) : expr)
+#eval (`(λx : ℕ, x + x) : expr)
+
+/- 1.4. Compare your answer with `expr.to_raw_fmt`. -/
+
+
+/- Question 2: `destruct_and` on steroids -/
+
+/- Recall from the lecture that `destruct_and` fails on the following easy goal: -/
+
+example {a b c d : Prop} (h : a ∧ (b ∧ c) ∧ d) : b ∧ d := sorry
+
+/- We will now address this by developing a new tactic called `destro_and`, which applies both
+*des*truction and in*tro*duction rules for conjunction. It will also go automatically through the
+hypotheses instead of taking an argument. We will develop it in three steps. -/
+
+/- 2.1. Develop a tactic `intro_ands` that replaces all goals of the form `a ∧ b` with two new goals
+`a` and `b` systematically, until all top-level conjunctions are gone.
+
+For this, we can use tactics such as `repeat` (which repeatedly applies a tactic on all goals until
+the tactic fails on each of the goal) and `applyc` (which can be used to apply a rule, in connection
+with backtick quoting). -/
+
+meta def intro_ands : tactic unit :=
+sorry
+
+example {a b c d : Prop} (h : a ∧ (b ∧ c) ∧ d) : b ∧ d :=
+begin
+  intro_ands,
+  /- The proof state should be as follows:
+
+  2 goals
+  a b c d : Prop,
+  h : a ∧ (b ∧ c) ∧ d
+  ⊢ b
+
+  a b c d : Prop,
+  h : a ∧ (b ∧ c) ∧ d
+  ⊢ d -/
+  repeat { sorry }
+end
+
+example {a b c d : Prop} (h : a ∧ (b ∧ c) ∧ d) : b ∧ (a ∧ (c ∧ b)) :=
+begin
+  intro_ands,
+  /- The proof state should be as follows:
+
+  4 goals
+  a b c d : Prop,
+  h : a ∧ (b ∧ c) ∧ d
+  ⊢ b
+
+  a b c d : Prop,
+  h : a ∧ (b ∧ c) ∧ d
+  ⊢ a
+
+  a b c d : Prop,
+  h : a ∧ (b ∧ c) ∧ d
+  ⊢ c
+
+  a b c d : Prop,
+  h : a ∧ (b ∧ c) ∧ d
+  ⊢ b -/
+  repeat { sorry }
+end
+
+/- 2.2. Develop a tactic `destruct_ands` that replaces hypotheses of the form `h : a ∧ b` by two new
+hypotheses `h_left : a` and `h_right : b` systematically, until all top-level conjunctions are gone.
+
+Here is imperative-style pseudocode that you can follow:
+
+1. Retrieve the list of hypotheses from the context. This is provided by the metaconstant
+`local_context`.
+
+2. Find the first hypothesis (= term) with a type (= proposition) of the form `_ ∧ _`. Here, you can
+use the `list.mfirst` function, in conjunction with pattern matching. You can use `infer_type` to
+query the type of a term.
+
+3. Perform a case split on the first found hypothesis. This can be achieved using the `cases`
+metafunction.
+
+4. Go to step 1.
+
+The above procedure might fail if there exists no hypotheses of the required form. Make sure to
+handle this failure gracefully using `<|>`. -/
+
+meta def destruct_ands : tactic unit :=
+sorry
+
+example {a b c d : Prop} (h : a ∧ (b ∧ c) ∧ d) : b ∧ d :=
+begin
+  destruct_ands,
+  /- The proof state should be as follows:
+
+  a b c d : Prop,
+  h_left : a,
+  h_right_right : d,
+  h_right_left_left : b,
+  h_right_left_right : c
+  ⊢ b ∧ d -/
+  sorry
+end
+
+/- 2.3. Finally, combine the two tactics developed above and the `assumption` tactic to implement
+the desired `destro_and` tactic. -/
+
+meta def destro_and : tactic unit :=
+sorry
+
+example {a b c d : Prop} (h : a ∧ (b ∧ c) ∧ d) : b ∧ d := by destro_and
+example {a b c d : Prop} (h : a ∧ (b ∧ c) ∧ d) : b ∧ (a ∧ (c ∧ b)) := by destro_and
+
+
+/- Question 3: A theorem finder -/
+
+/- We will implement a function that allows us to find theorems by constants appearing in their
+statements. So given a list of constant names, the function will list all theorems in which all
+these constants appear.
+
+You can use the following metaconstants:
+
+* `declaration`: contains all data (name, type, value) associated with a declaration,
+  i.e. axiom, theorem, constant, etc.
+* `tactic.get_env`: gives us access to the `environment`, a metatype thats lists all `declaration`s
+  (especially all theorems)
+* `environment.fold` allows us to walk through the environment and collect data
+* `expr.fold` allows us to walk through an expression and collect data. -/
+
+/- 3.1. Write a metafunction that checks whether an expression contains a specific constant.
+
+You can use `expr.fold` to walk through the expression, `||` and `ff` for Booleans, and
+`expr.is_constant_of` to check if an expression is a constant. -/
+
+meta def term_contains (e : expr) (n : name) : bool :=
+sorry
+
+/- 3.2. Write a metafunction that checks whether an expression contains _all_ constants in a list.
+
+You can use `list.band` (Boolean and). -/
+
+meta def term_contains_all (ns : list name) (e : expr) : bool :=
+sorry
+
+/- 3.3. Produce the list of all theorems that contain all constants `ns` in their statement.
+
+`environment.fold` allows you to walk over the list of declarations. With `declaration.type`, you
+get the type of a theorem, and with `declaration.to_name` you get the name. -/
+
+meta def list_constants (ns : list name) (e : environment) : list name :=
+sorry
+
+/- 3.4. Finally, develop a tactic that uses the above metafunctions to log all found theorems.
+
+You can use `trace` to log the results. -/
+
+meta def find_constants (ns : list name) : tactic unit :=
+sorry
+
+/- 3.5. Test your solution. -/
+
+run_cmd find_constants []  -- lists all theorems
+run_cmd find_constants [`list.map, `function.comp]
