24_lecture.lean
@@ -1,0 +1,179 @@
+/- Lecture 2.4: Functional Programming — Metaprogramming -/
+
+/- Tactics -/
+
+example : true :=
+  by tactic.triv
+
+example : true := by do
+  tactic.trace "Hello, Metacosmos!",
+  tactic.triv
+
+meta def hello_world : tactic unit := do
+  tactic.trace "Hello, Metacosmos!",
+  tactic.triv
+
+example : true := by hello_world
+
+run_cmd hello_world
+
+open tactic
+
+example (α : Type) (a : α) : true := by do
+  trace "local context:",
+    local_context >>= trace,
+  trace "goals:",
+    get_goals >>= trace,
+  trace "target:",
+    target >>= trace,
+  triv
+
+meta def exact_list : list expr → tactic unit
+| []        := fail "no matching expression found"
+| (e :: es) :=
+  (do
+    trace "trying ",
+    trace e,
+    exact e)
+  <|> exact_list es
+
+meta def find_assumption : tactic unit := do
+  es ← local_context,
+  exact_list es
+
+example {p : Prop} {α : Type} (a : α) (h : p) : p := by do
+  find_assumption
+
+example {p : Prop} (h : p) : p := by do
+  p_proof ← get_local `h,
+  trace "p_proof:",
+    trace p_proof,
+    trace p_proof.to_raw_fmt,
+  trace "type of p_proof:",
+    infer_type p_proof >>= trace,
+  trace "type of type of p_proof:",
+    infer_type p_proof >>= infer_type >>= trace,
+  apply p_proof
+
+
+/- Names and expressions -/
+
+#print expr
+
+#check expr tt  -- elaborated expressions
+#check expr ff  -- unelaborated expressions (pre-expressions)
+
+#print name
+
+#check (expr.const `ℕ [] : expr)
+
+#check expr.sort level.zero  -- Sort 0, i.e. Prop
+#check expr.sort (level.succ level.zero)  -- Sort 1, i.e. Type 0 (Type)
+
+#check expr.app
+#check expr.var 0  -- bound variable of De Bruijn index 0
+#check (expr.local_const `uniq_name `pp_name binder_info.default `(ℕ) : expr)
+#check (expr.mvar `uniq_name `pp_name `(ℕ) : expr)
+#check (expr.pi `pp_name binder_info.default `(ℕ) (expr.sort level.zero) : expr)
+#check (expr.lam `pp_name binder_info.default `(ℕ) (expr.var 0) : expr)
+#check expr.elet
+#check expr.macro
+
+
+/- Name literals -/
+
+run_cmd trace `name.a
+run_cmd trace ``true
+run_cmd trace ``name.a -- not found
+
+
+/- Expression literals -/
+
+-- one backtick: fully elaborated expressions (using reflection)
+
+run_cmd do
+  let e : expr := `(list.map (λn : ℕ, n + 1) [1, 2, 3]),
+  trace e
+
+run_cmd do
+  let e : expr := `(list.map _ [1, 2, 3]),  -- error: holes not allowed
+  skip
+
+-- two backticks: checked pre-expressions
+
+run_cmd do
+  let e₀ : pexpr := ``(list.map (λn, n + 1) [1, 2, 3]),
+  let e₁ : pexpr := ``(list.map _ [1, 2, 3]),
+  trace e₀,
+  trace e₁
+
+-- three backticks: pre-expressions without name checking
+
+run_cmd do
+  let e := ```(a),
+  trace e
+
+
+/- Antiquotations -/
+
+run_cmd do
+  let x : expr := `(2 : ℕ),
+  let e : expr := `(%%x + 1),
+  trace e
+
+run_cmd do
+  let x : expr := `(@id ℕ),
+  let e := ``(list.map %%x),
+  trace e
+
+run_cmd do
+  let x : expr := `(@id ℕ),
+  let e := ```(a _ %%x),
+  trace e
+
+
+/- Pattern matching -/
+
+example : 1 + 2 = 3 := by do
+  `(%%a + %%b = %%r) ← target,
+  trace a, trace b, trace r,
+  `(@eq %%α %%l' %%r') ← target,
+  trace α, trace l', trace r',
+  exact `(refl _ : 3 = 3)
+
+
+/- A simple tactic: `destruct_and` -/
+
+example {a b c d : Prop} (h : a ∧ (b ∧ c) ∧ d) : a := and.left h
+example {a b c d : Prop} (h : a ∧ (b ∧ c) ∧ d) : b := and.left (and.left (and.right h))
+example {a b c d : Prop} (h : a ∧ (b ∧ c) ∧ d) : b ∧ c := and.left (and.right h)
+
+-- `destruct_and_core t h` uses the conjunction `h : t` to prove the current goal
+meta def destruct_and_core : expr → expr → tactic unit
+| `(%%a ∧ %%b) h :=
+    exact h
+    <|> (to_expr ``(and.left %%h) >>= destruct_and_core a)
+    <|> (to_expr ``(and.right %%h) >>= destruct_and_core b)
+| _            h := exact h
+
+meta def destruct_and (h : name) : tactic unit := do
+  h ← get_local h,
+  t ← infer_type h,
+  destruct_and_core t h
+
+example {a b c d : Prop} (h : a ∧ (b ∧ c) ∧ d) : a := by destruct_and `h
+example {a b c d : Prop} (h : a ∧ (b ∧ c) ∧ d) : b := by destruct_and `h
+example {a b c d : Prop} (h : a ∧ (b ∧ c) ∧ d) : b ∧ c := by destruct_and `h
+example {a b c d : Prop} (h : a ∧ (b ∧ c) ∧ d) : b ∧ d := by destruct_and `h  -- fails
+
+#check exact
+#check interactive.exact
+#check lean.parser
+
+open interactive.types
+
+meta def tactic.interactive.destruct_and (h : interactive.parse ident_) : tactic unit :=
+destruct_and h
+
+example {a b c d : Prop} (h : a ∧ (b ∧ c) ∧ d) : a :=
+by destruct_and h
