Exercises 7/24_homework_sheet.lean
@@ -1,0 +1,236 @@
+/- Homework 2.4: Functional Programming — Metaprogramming -/
+
+open expr
+open tactic
+open declaration
+
+
+/- Question 1: A `safe` tactic -/
+
+/- We develop a tactic that applies all safe introduction and elimination rules for the connectives
+and quantifiers exhaustively. A rule is said to be _safe_ if it always gives rise to provable
+subgoals. In addition, we will require that safe rules do not introduce metavariables (which can
+easily be instantiated accidentally with the wrong terms.) We proceed in three steps. -/
+
+/- 1.1. Develop a `safe_intros` tactic that applies the introduction rules for `true', `¬`, `∧`,
+`↔`, and `→`/`∀`. (Hint: You can use `tactic.intro` or `tactic.intro1` for some of these.) -/
+
+meta def safe_intros : tactic unit :=
+sorry
+
+example {a b c d e f : Prop} {p : ℕ → Prop} : a → ¬ b ∧ (c ↔ d) :=
+begin
+  safe_intros,
+  /- The proof state should be roughly as follows:
+
+  a b c d e f : Prop,
+  p : ℕ → Prop,
+  a_1 : a,
+  a_2 : b
+  ⊢ false
+
+  a b c d e f : Prop,
+  p : ℕ → Prop,
+  a_1 : a,
+  a_2 : c
+  ⊢ d
+
+  a b c d e f : Prop,
+  p : ℕ → Prop,
+  a_1 : a,
+  a_2 : d
+  ⊢ c -/
+  repeat { sorry }
+end
+
+/- 1.2. Develop a `safe_destructs` tactic that eliminates `false`, `∧`, `∨`, `↔`, and `∃`. -/
+
+meta def safe_destructs : tactic unit :=
+sorry
+
+example {a b c d e f : Prop} {p : ℕ → Prop}
+  (hneg: ¬ a) (hand : a ∧ b ∧ c) (hor : c ∨ d) (himp : b → e) (hiff : e ↔ f) (hex : ∃x, p x) :
+  false :=
+begin
+  safe_destructs,
+  /- The proof state should be roughly as follows:
+
+  2 goals
+  a b c d e f : Prop,
+  p : ℕ → Prop,
+  hneg : ¬a,
+  himp : b → e,
+  hand_left : a,
+  hor : c,
+  hiff_mp : e → f,
+  hiff_mpr : f → e,
+  hex_w : ℕ,
+  hex_h : p hex_w,
+  hand_right_left : b,
+  hand_right_right : c
+  ⊢ false
+
+  a b c d e f : Prop,
+  p : ℕ → Prop,
+  hneg : ¬a,
+  himp : b → e,
+  hand_left : a,
+  hor : d,
+  hiff_mp : e → f,
+  hiff_mpr : f → e,
+  hex_w : ℕ,
+  hex_h : p hex_w,
+  hand_right_left : b,
+  hand_right_right : c
+  ⊢ false -/
+  repeat { sorry }
+end
+
+/- 1.3. Implement a `safe` tactic that first performs introduction, then elimination, and finally
+proves all the subgoals that can be discharged directly by `assumption`.
+
+Hint: The `try` tactic combinator might come in handy. -/
+
+meta def safe : tactic unit :=
+sorry
+
+example {a b c d e f : Prop} {p : ℕ → Prop}
+(hneg: ¬ a) (hand : a ∧ b ∧ c) (hor : c ∨ d) (himp : b → e) (hiff : e ↔ f) (hex : ∃x, p x) :
+  a → ¬ b ∧ (c ↔ d) :=
+begin
+  safe,
+  /- The proof state should be roughly as follows:
+
+  3 goals
+  a b c d e f : Prop,
+  p : ℕ → Prop,
+  hneg : ¬a,
+  himp : b → e,
+  a_1 : a,
+  a_2 : b,
+  hand_left : a,
+  hor : c,
+  hiff_mp : e → f,
+  hiff_mpr : f → e,
+  hex_w : ℕ,
+  hex_h : p hex_w,
+  hand_right_left : b,
+  hand_right_right : c
+  ⊢ false
+
+  a b c d e f : Prop,
+  p : ℕ → Prop,
+  hneg : ¬a,
+  himp : b → e,
+  a_1 : a,
+  a_2 : b,
+  hand_left : a,
+  hor : d,
+  hiff_mp : e → f,
+  hiff_mpr : f → e,
+  hex_w : ℕ,
+  hex_h : p hex_w,
+  hand_right_left : b,
+  hand_right_right : c
+  ⊢ false
+
+  a b c d e f : Prop,
+  p : ℕ → Prop,
+  hneg : ¬a,
+  himp : b → e,
+  a_1 : a,
+  a_2 : c,
+  hand_left : a,
+  hor : c,
+  hiff_mp : e → f,
+  hiff_mpr : f → e,
+  hex_w : ℕ,
+  hex_h : p hex_w,
+  hand_right_left : b,
+  hand_right_right : c
+  ⊢ d -/
+  repeat { sorry }
+end
+
+
+/- Question 2: A `solve_direct` advisor -/
+
+/- It often happens that a user states a new lemma, proves it, and later realizes that the lemma
+already exists in the library. To help prevent this, we want to implement a `solve_direct` tactic,
+which goes through all lemmas in the database and checks whether one of them can be used to fully
+solve the statement. We implement it in steps. -/
+
+/- 2.1. Develop a function that returns `tt` if a `declaration` is a theorem (`declaration.thm`) or
+an axiom (`declaration.ax`) and `ff` otherwise. -/
+
+meta def is_theorem : declaration → bool
+:= sorry
+
+/- 2.2. Develop a function that returns the list of all theorem names (theorem in the sense of
+`is_theorem`).
+
+Here `get_env` and `environment.fold` are very helpful. See also Question 3 of the exercise. -/
+
+meta def get_all_theorems : tactic (list name) :=
+sorry
+
+/- 2.3. Develop a tactic that (fully) solves the goal using a theorem `n`.
+
+Hints:
+
+* `mk_const n` can be used to produce an `expr` (representing the proof) from a name `n` (the
+theorem name).
+
+* `apply` applies an `expr` to the current goal. For speed reasons one might want to add the
+c onfiguration `apply c { md := transparency.reducible, unify := ff }`, where `c : expr` is the
+current theorem, and the parameters in `{ ... }` tell `apply` to apply less computational unfolding.
+
+* `all_goals` in combination with `assumption` can be used to ensure that the hypothesis from the
+local context are used to fill in all remaining subgoals.
+
+* `done` can be used to check that no subgoal is left. -/
+
+meta def solve (n : name) : tactic unit :=
+sorry
+
+/- 2.4. Implement `solve_direct`.
+
+Now `solve_direct` should go through `get_all_theorems` and succeed with the first theorem solving
+the current goal.
+
+You can use `list.mfirst` to apply a tactic to each element of a list until one application
+succeeds. Use `trace` to output the successful theorem to the user. -/
+
+meta def solve_direct : tactic unit :=
+sorry
+
+/- 2.5. Develop a version of `solve_direct` that also looks for equalities stated in symmetric form
+(e.g., if the goal is `l = r` but the theorem is `r = l`). -/
+
+#check eq.symm
+
+meta def solve_direct_symm : tactic unit :=
+sorry
+
+example {n : ℕ} : n + 0 = n := by solve_direct_symm
+example {n : ℕ} : n = n + 0 := by solve_direct_symm
+
+
+/- Question 3 **optional**: An `auto` tactic -/
+
+/- 3.1. Develop an Isabelle-style `auto` tactic.
+
+This tactic would apply all safe introduction and elimination rules. In addition, it would try
+unsafe rules (such as `or.intro_left` and `false.elim`) but backtrack at some point
+(or try several possibilities in parallel). Iterative deepening may be a valid approach, or
+best-first search, or breadth-first search. The tactic should also attempt to apply assumptions
+whose conclusion matches the goal, but backtrack if necessary.
+
+See also "Automatic Proof and Disproof in Isabelle/HOL"
+(https://www.cs.vu.nl/~jbe248/frocos2011-dis-proof.pdf) by Blanchette, Bulwahn, and Nipkow, and the
+references they give. -/
+
+/- 3.2. Test your tactic on some benchmarks.
+
+You can try your tactic on logical puzzles of the kinds we proved in exercise 1.3 and howework 1.3.
+Please include these below. -/
